Now we just have to find the point of intersection of all the labels of each of the 2, 3, or 5 labels and clamp (by *) that point on top of the other 2 or 3 labels:

$$\int\frac{2}{3!} P(2,3,5)=((2,3,5),(2,3,1),(2,3,0)\wedge((3,0,0)$$

*You may have noticed that while the intersection of all the labels must be the same (i.e all \(w\)'s must be either positive or negative) this doesn't necessarily hold true for the rest of the equations. In particular the solution set for $\mu(x)=0$ along with the solution set for $\mu(y)=1$ along with the entire solution set for $\mu(x\to y)=\omega$.*

Now we just have to find the $\mathbb{R}$ of each of the 2, 3, 5, or 7 (logarithmic) equations and clamp it to the other equations:

$$\mathbb{R}^2=\begin{pmatrix} (2,3,5,1) & (2,3,5,0) & \ \ \ (2,3,5,-1) \\ (3,3,5,0,1) & (3,3,5,0,1) & \ \ \ (3,3,5,1,0) \\ (5,3,5,0,1) & (5,3,5,0,1) & \ \ \ (5,3,5,0,1,0) \\ (7,3,5,0,1) & (7,3,5,0,1) & \ \ \ (7,3,5,0,1,0)
\end{pmatrix}$$

And using the ratio we found earlier, we can calculate the $-1$:

$$-1:\frac{w-1}{2!} W\iff\frac{w}{2}=t$$

We can plug all these values into our original formula and it will return the desired ratio:

$$\begin{align}
\mu(x)&=\frac{w}{2}\left(x-\frac{2}{3}+\cdots+\frac{w}{2}\right)\\
&=\frac{w^2}{2!} W \iff \frac{2}{3}=t\\
&=\frac{\pi}{4}t+\cdots+\frac{\pi}{2}t\\
&=\frac{\pi}{2}t+\cdots+ \cdots+ \cdots+ \cdots+ \cdots+ \cdots+ \cdots+ \cdots+ \cdots+ \cdots+ \cdots+ \cdots+ \cdots+ \cdots+ \ddots+ \cdots+ \cdots+ \cdots+ \vdots+ \ddots+ \cdots+ \cdots+ \vdots+ \vdots+ \vdots+ \vdots+ \vdots+ \vdots+ \vdots+ \vdots+\vdots+\vdots+\vdots+\vdots+\vdots+\vdots+\vdots+\vdots+\vdots
\end{align}$$

Here we can see the rule of sum is repeated for each vector in the Cartesian product.

With the $\pi$ terms reversed we can form the formula more succinctly:

$$\begin{align}
&\phantom{\pi 0}\\
&=\frac{\pi}{2}-\frac{\pi}{2}\\
&=\frac{\pi}{2}-\frac{\pi}{2}\\
&=\frac{\pi}{2}-0\\
\end{align}$$

This is all there is to it. Plugging the values from the Cartesian product back into the differential equation and seeing what the correct answer is we finally arrive at:

$$\left(\frac{\pi}{2}\right) \left(\frac{\pi}{2} \text{ Conjugates} \right)=\frac{\pi}{2}$$

We only needed to find the third derivative of $x$ to solve the above equation. Enter the powers of both sides and differential equation: